Create solver for mutable
Fixes #13

theories/Handlers/Mutable.v
@@ -1,6 +1,9 @@
 From Coq Require Import
      List.
 
+From Equations Require Import
+     Equations.
+
 Import ListNotations.
 
 From LibTx Require Import
@@ -20,7 +23,7 @@ Section defs.
     | _   => True
     end.
 
-  Let ctx := mkCtx PID req_t ret_t.
+  Definition ctx := mkCtx PID req_t ret_t.
   Let TE := @TraceElem ctx.
 
   Notation "pid '@' ret '<~' req" := (@trace_elem ctx pid req ret).
@@ -39,14 +42,73 @@ Section defs.
       h_chain_rule := mut_chain_rule;
     |}.
 
+  Lemma mut_get_rewr : forall s s' pid ret,
+      mut_chain_rule s s' (pid @ ret <~ get) ->
+      s = s' /\ ret = s.
+  Proof.
+    intros.
+    remember (pid @ ret <~ get) as te.
+    inversion H.
+    - subst te.
+      inversion H2. subst pid.
+      apply te_ret_eq in H2.
+      firstorder.
+    - now subst.
+  Qed.
+
+  Lemma mut_put_rewr : forall s s' pid v,
+      mut_chain_rule s s' (pid @ I <~ put v) ->
+      v = s'.
+  Proof.
+    intros.
+    remember (pid @ I <~ put v) as te.
+    inversion H.
+    - now subst.
+    - subst.
+      now inversion H2.
+  Qed.
+
   Fail Lemma mut_get_comm : forall v pid1 pid2, (*TODO*)
       trace_elems_commute (trace_elem ctx pid1 get v) (trace_elem ctx pid2 get v).
 End defs.
 
 Ltac elim_mut :=
-  repeat match goal with
-           [H: mut_chain_rule _ _ ?s ?s' ?te |- _] =>
-           inversion_clear H;
-           try subst s;
-           try subst s'
-         end.
+  match goal with
+  | [H: mut_chain_rule ?PID ?T ?s ?s' ?te |- _] =>
+    lazymatch eval cbn in te with
+    | trace_elem _ ?pid get ?ret =>
+      apply mut_get_rewr in H;
+      let H1 := fresh "H" in
+      let H2 := fresh "H" in
+      destruct H as [H1 H2];
+      subst s';
+      subst ret
+    | trace_elem _ ?pid (put ?v) ?ret =>
+      try destruct ret;
+      apply (mut_put_rewr PID T s s' pid) in H;
+      subst s'
+    end
+  end.
+
+Hint Extern 4 => elim_mut : handlers.
+
+Section tests.
+  Let PID := True.
+  Let handler := t PID nat (fun s => s = 0).
+  Let ctx := ctx PID nat.
+  Notation "pid '@' ret '<~' req" := (trace_elem ctx pid req ret).
+
+  Goal forall s s' pid ret,
+      mut_chain_rule _ _ s s' (pid @ ret <~ get) -> s = ret.
+  Proof.
+    intros.
+    auto with handlers.
+  Qed.
+
+  Goal forall s s' pid v,
+      mut_chain_rule _ _ s s' (pid @ I <~ put v) -> s' = v.
+  Proof.
+    intros.
+    auto with handlers.
+  Qed.
+End tests.
