theories/SLOT/EventTrace.v
@@ -1,5 +1,15 @@
 From Coq Require Import
-     List.
+     List
+     Logic.EqdepFacts.
+
+From Equations Require Import
+     Equations.
+
+Let transp {A} {B : A -> Type} {x y : A} (e : x = y) : B x -> B y :=
+  fun bx => eq_rect x B bx y e.
+
+Let ap {A B} (f : A -> B) {x y : A} : x = y -> f x = f y.
+Proof. now intros ->. Defined.
 
 Reserved Notation "pid '@' req '<~' ret" (at level 30).
 
@@ -14,7 +24,13 @@ Record TraceElem {ctx : Ctx} : Set :=
                te_req : ctx_req_t ctx;
                te_ret : (ctx_ret_t ctx) te_req;
              }.
+Derive NoConfusionHom for TraceElem.
 
 Definition Trace {ctx : Ctx} := list (@TraceElem ctx).
 
 Notation "pid '@' req '<~' ret" := (trace_elem _ pid req ret).
+
+Lemma te_ret_eq : forall ctx pid req ret1 ret2,
+    trace_elem ctx pid req ret1 = trace_elem ctx pid req ret2 ->
+    ret1 = ret2.
+Admitted. (* TODO *)
